# 文法
### S                                    ------>             <程序>

### <程序>                          ------>               main()<语句块>

### <语句块>                   ---------->                       '{'<语句串'}'

### <语句串>                      -------->         <语句串> <语句>;

### <语句串>                    -------->          <语句>;

### <语句>                    ------------>          <赋值语句> 

### <语句>                    ------------>          <条件语句> 

### <语句>                    ------------>          <循环语句>

### <赋值语句>               ----------->            ID = <表达式>

### <赋值语句>               ----------->           int' 'ID = <表达式>

### <条件语句>               ----------->            if(<布尔语句>)<语句块>

### <条件语句>               ----------->            if(<布尔语句>)<语句块><分支语句>

### <分支语句>               ----------->            else<条件语句>

### <分支语句>               ----------->            else<语句块>

### <布尔语句>               ----------->            <表达式><关系运算符><表达式>

### <表达式>                   ----------->            <项> 

### <表达式>                   ----------->            <项>  +  <项>

### <表达式>                   ----------->            <项>  -  <项>

### <项>                          ----------->            <因子>  

### <项>                          ----------->            <因子>  * <因子>

### <项>                          ----------->            <因子>  / <因子>

### <因子>                          ----------->          ID

### <因子>                          ----------->          NUM

### <因子>                          ----------->          (<表达式>)

### <关系运算符>               ----------->          >=|<=|==|<|>



# 项目

### (0) S  --->    ·<程序>

### (1) S  --->    <程序>·

### (2) <程序>  --->  ·main()<语句块>

### (3) <程序>  ---->  main·()<语句块>

### (4) <程序>  ---->  main(·)<语句块>

### (5) <程序>  ---->  main()·<语句块>

### (6) <程序>  ---->  main()<语句块>·

### (6) <语句块>  ----> ·'{'<语句串>'}'

### (6) <语句块>  ----> '{'·<语句串>'}'

### (6) <语句块>  ----> '{'<语句串>·'}'

### (6) <语句块>  ----> '{'<语句串>'}'·

### (6) <语句串>  ----> ·<语句串><语句>;

### (6) <语句串>  ----> <语句串>·<语句>;

### (6) <语句串>  ----> <语句串><语句>·;

### (6) <语句串>  ----> <语句串><语句>;·

### (6) <语句串>  ----> ·<语句>;

### (6) <语句串>  ----> <语句>·;

### (6) <语句串>  ----> <语句>;·

### (6) <语句>  ----> <赋值语句>















































